EnumeratedDistributesOverConcat!

src/Actions/FilteredEnumerator.dfy
@@ -54,9 +54,12 @@ module Filtered {
     ghost predicate CanProduce(consumed: seq<()>, produced: seq<Option<T>>)
       decreases height
     {
-      exists producedByWrapped: seq<Option<T>> ::
-        && wrappedCanProduce(Seq.Repeat((), |producedByWrapped|), producedByWrapped)
-        && Enumerated(produced) == Seq.Filter(filter, Enumerated(producedByWrapped))
+      exists producedByWrapped: seq<Option<T>> :: ValidWrappedProduced(produced, producedByWrapped)
+    }
+
+    ghost predicate ValidWrappedProduced(produced: seq<Option<T>>, producedByWrapped: seq<Option<T>>) {
+      && wrappedCanProduce(Seq.Repeat((), |producedByWrapped|), producedByWrapped)
+      && Enumerated(produced) == Seq.Filter(filter, Enumerated(producedByWrapped))
     }
 
     method {:vcs_split_on_every_assert} Invoke(t: ()) returns (r: Option<T>) 
@@ -72,6 +75,7 @@ module Filtered {
       while true
         invariant wrapped.Valid()
         invariant fresh(wrapped.Repr - old(wrapped.Repr))
+        invariant ValidWrappedProduced(produced, wrapped.produced)
         invariant produced == old(produced)
         invariant consumed == old(consumed)
         invariant Enumerated(produced) == Seq.Filter(filter, Enumerated(wrapped.produced))
@@ -89,23 +93,34 @@ module Filtered {
         if r.None? || filter(r.value) {
           break;
         }
-
-        var wrappedEnumeratedBefore := Enumerated(old@before(wrapped.produced));
-        assert wrapped.produced == old@before(wrapped.produced) + [r];
-
-        ProducingSomeImpliesTerminated@before(wrapped, r);
-        TerminatedBoundsEnumerated(wrapped.produced, |wrapped.produced|);
-        // TerminatedDistributesOverConcat(old@before(wrapped.produced), [r], None, 1);
-        assert |Enumerated(wrapped.produced)| == |wrapped.produced|;
-        assert wrapped.produced == old@before(wrapped.produced) + [r];
-        EnumeratedDistributesOverConcat(old@before(wrapped.produced), [r], 1);
-        assert Enumerated(wrapped.produced) == Enumerated(old@before(wrapped.produced)) + [r.value];
-        LemmaFilterDistributesOverConcat(filter, wrappedEnumeratedBefore, [r.value]);
-        assert Enumerated(produced) == Seq.Filter(filter, Enumerated(wrapped.produced));
-
         EnumerationTerminationMetricDecreased@before(wrapped, r);
+
+        // var wrappedEnumeratedBefore := Enumerated(old@before(wrapped.produced));
+        // assert wrapped.produced == old@before(wrapped.produced) + [r];
+
+        // ProducingSomeImpliesTerminated@before(wrapped, r);
+        // TerminatedBoundsEnumerated(wrapped.produced, |wrapped.produced|);
+        // // TerminatedDistributesOverConcat(old@before(wrapped.produced), [r], None, 1);
+        // assert |Enumerated(wrapped.produced)| == |wrapped.produced|;
+        // assert wrapped.produced == old@before(wrapped.produced) + [r];
+        // EnumeratedDistributesOverConcat(old@before(wrapped.produced), [r], 1);
+        // assert Enumerated(wrapped.produced) == Enumerated(old@before(wrapped.produced)) + [r.value];
+        
+        // assert Enumerated(old(produced)) == Seq.Filter(filter, Enumerated(old(wrapped.produced)));
+        // calc {
+        //   Seq.Filter(filter, Enumerated(wrapped.produced));
+        //   Seq.Filter(filter, Enumerated(old(wrapped.produced) + [r]));
+        //   Seq.Filter(filter, Enumerated(old(wrapped.produced)) + Enumerated([r]));
+        //   Seq.Filter(filter, Enumerated(old(wrapped.produced)) + [r.value]);
+        //   { LemmaFilterDistributesOverConcat(filter, wrappedEnumeratedBefore, [r.value]); }
+        //   Seq.Filter(filter, Enumerated(old(wrapped.produced))) + Seq.Filter(filter, [r.value]);
+        //   Seq.Filter(filter, Enumerated(old(wrapped.produced)));
+        // }
+        // assert Enumerated(produced) == Seq.Filter(filter, Enumerated(wrapped.produced));
       }
 
+      assert r.Some? ==> filter(r.value);
+      assert wrapped.CanProduce(wrapped.consumed, wrapped.produced);
       Update(t, r);
     }
   }
