src/Actions/Actions.dfy
@@ -62,73 +62,18 @@ module Actions {
     forall i | 0 <= i < |s| :: n <= i <==> s[i] == c
   }
 
+  lemma TerminatedMinConcat<T>(left: seq<T>, right: seq<T>, c: T, n: nat, m: nat) 
+    requires Terminated(left, c, n)
+    requires Terminated(left + right, c, m)
+    ensures n < m
+  {
+
+  }
+
   ghost predicate ProducesTerminatedBy<T(!new), R(!new)>(i: Action<T, R>, c: R, n: nat) {
     forall consumed: seq<T>, produced: seq<R> ::
       i.CanProduce(consumed, produced) ==> Terminated(produced, c, n)
   }
-
-  // class Compose<T, V(!new), R> extends Action<T, R> {
-
-  //   const first: Action<T, V>
-  //   const second: Action<V, R>
-
-  //   ghost predicate Valid() 
-  //     reads this, Repr 
-  //     ensures Valid() ==> this in Repr 
-  //     ensures Valid() ==> 
-  //       && CanProduce(consumed, produced)
-  //     decreases Repr, 0
-  //   {
-  //     && this in Repr
-  //     && ValidComponent(first)
-  //     && ValidComponent(second)
-  //     && CanProduce(consumed, produced)
-  //   }
-
-  //   constructor(second: Action<V, R>, first: Action<T, V>) 
-  //     requires first.Valid()
-  //     requires second.Valid()
-  //     requires first.Repr !! second.Repr
-  //     requires first.CanProduce([], [])
-  //     requires second.CanProduce([], [])
-  //     ensures Valid()
-  //     ensures produced == []
-  //   { 
-  //     this.first := first;
-  //     this.second := second;
-
-  //     consumed := [];
-  //     produced := [];
-  //     Repr := {this} + first.Repr + second.Repr;
-  //   }
-
-  //   ghost predicate CanConsume(consumed: seq<T>, produced: seq<R>, next: T) {
-  //     exists vs: seq<V> :: 
-  //       && first.CanProduce(consumed, vs)
-  //       && first.CanConsume(consumed, vs, next)
-  //   }
-  //   ghost predicate CanProduce(consumed: seq<T>, produced: seq<R>) {
-  //     exists vs: seq<V> :: first.CanProduce(consumed, vs) && second.CanProduce(vs, produced)
-  //   }
-
-  //   method Invoke(t: T) returns (r: R) 
-  //     requires Valid()
-  //     requires CanConsume(consumed, produced, t)
-  //     modifies Repr
-  //     decreases Repr
-  //     ensures Valid()
-  //     ensures Repr <= old(Repr)
-  //     ensures consumed == old(consumed) + [t]
-  //     ensures produced == old(produced) + [r]
-  //     ensures CanProduce(consumed, produced)
-  //   {
-  //     var v := first.Invoke(t);
-  //     r := second.Invoke(v);
-
-  //     Update(t, r);
-  //   }
-
-  // }
 
   type IAggregator<T> = Action<T, ()>
   type Aggregator<T(!new)> = a: Action<T, bool> | exists n :: ProducesTerminatedBy(a, false, n) witness *
@@ -216,56 +161,6 @@ module Actions {
       storage[..index]
     }
   }
-
-  // class SeqEnumerator<T> extends Action<(), Option<T>> {
-
-  //   const elements: seq<T>
-  //   var index: nat
-
-  //   ghost predicate Valid() 
-  //     reads this, Repr 
-  //     ensures Valid() ==> this in Repr 
-  //     ensures Valid() ==> 
-  //       && CanProduce(consumed, produced)
-  //     decreases Repr, 0
-  //   {
-  //     && this in Repr
-  //     && 0 <= index <= |elements|
-  //     && Enumerated(produced) == elements[0..index]
-  //   }
-
-  //   constructor(s: seq<T>) 
-  //     ensures Valid()
-  //     ensures fresh(Repr - {this})
-  //     ensures produced == []
-  //     ensures elements == s
-  //   {
-  //     elements := s;
-  //     index := 0;
-      
-  //     consumed := [];
-  //     produced := [];
-  //     Repr := {this};
-  //   }
-
-  //   ghost predicate CanConsume(toConsume: seq<()>, produced: seq<Option<T>>, next: ()) {
-  //     true
-  //   }
-  //   ghost predicate CanProduce(consumed: seq<()>, toProduce: seq<Option<T>>) {
-  //     toProduce == ProducedForEnumerator(elements, |consumed|)
-  //   }
-
-  //   method Invoke(t: ()) returns (r: Option<T>) 
-  //     requires Valid()
-  //     requires CanConsume(consumed, produced, t)
-  //     ensures Valid()
-  //     ensures consumed == old(consumed) + [t]
-  //     ensures produced == old(produced) + [r]
-  //     ensures CanProduce(consumed, produced)
-  //   {
-
-  //   }
-  // }
 
   method AggregatorExample() {
     var a := new ArrayAggregator();
