src/Actions/ComposedAction.dfy
@@ -1,0 +1,70 @@
+
+include "Actions.dfy"
+
+module Composed {
+
+  import opened Actions
+
+  class Compose<T, V(!new), R> extends Action<T, R> {
+
+    const first: Action<T, V>
+    const second: Action<V, R>
+
+    ghost predicate Valid() 
+      reads this, Repr 
+      ensures Valid() ==> this in Repr 
+      ensures Valid() ==> 
+        && CanProduce(consumed, produced)
+      decreases Repr, 0
+    {
+      && this in Repr
+      && ValidComponent(first)
+      && ValidComponent(second)
+      && CanProduce(consumed, produced)
+    }
+
+    constructor(second: Action<V, R>, first: Action<T, V>) 
+      requires first.Valid()
+      requires second.Valid()
+      requires first.Repr !! second.Repr
+      requires first.CanProduce([], [])
+      requires second.CanProduce([], [])
+      ensures Valid()
+      ensures produced == []
+    { 
+      this.first := first;
+      this.second := second;
+
+      consumed := [];
+      produced := [];
+      Repr := {this} + first.Repr + second.Repr;
+    }
+
+    ghost predicate CanConsume(consumed: seq<T>, produced: seq<R>, next: T) {
+      exists vs: seq<V> :: 
+        && first.CanProduce(consumed, vs)
+        && first.CanConsume(consumed, vs, next)
+    }
+    ghost predicate CanProduce(consumed: seq<T>, produced: seq<R>) {
+      exists vs: seq<V> :: first.CanProduce(consumed, vs) && second.CanProduce(vs, produced)
+    }
+
+    method Invoke(t: T) returns (r: R) 
+      requires Valid()
+      requires CanConsume(consumed, produced, t)
+      modifies Repr
+      decreases Repr
+      ensures Valid()
+      ensures Repr <= old(Repr)
+      ensures consumed == old(consumed) + [t]
+      ensures produced == old(produced) + [r]
+      ensures CanProduce(consumed, produced)
+    {
+      var v := first.Invoke(t);
+      r := second.Invoke(v);
+
+      Update(t, r);
+    }
+
+  }
+}
