src/Actions/MappingEnumerator.dfy
@@ -1,0 +1,90 @@
+
+include "Enumerators.dfy"
+
+module Mapped {
+
+  import opened Actions
+  import opened Enumerators
+  import opened Wrappers
+  import opened Seq
+
+  class Map<T(!new), R(!new)> extends Action<(), Option<R>> {
+
+    const wrapped: Action<(), Option<T>>
+    ghost const wrappedCanProduce: (seq<()>, seq<Option<T>>) -> bool
+      
+    // TODO: Can we support --> or ~>?
+    const f: T -> R
+
+    ghost predicate Valid() 
+      reads this, Repr 
+      ensures Valid() ==> this in Repr 
+      ensures Valid() ==> 
+        && CanProduce(consumed, produced)
+      decreases height, 0
+    {
+      && this in Repr
+      && ValidComponent(wrapped)
+      && IsEnumerator(wrapped)
+      && CanProduce(consumed, produced)
+      && Enumerated(produced) == Seq.Map(f, Enumerated(wrapped.produced))
+    }
+
+    constructor(f: T -> R, wrapped: Action<(), Option<T>>) 
+      requires wrapped.Valid()
+      requires IsEnumerator(wrapped)
+      requires wrapped.consumed == [] && wrapped.produced == []
+      ensures Valid()
+    { 
+      this.f := f;
+      this.wrapped := wrapped;
+
+      consumed := [];
+      produced := [];
+      Repr := {this} + wrapped.Repr;
+      height := wrapped.height + 1;
+      wrappedCanProduce := wrapped.CanProduce;
+    }
+
+    ghost predicate CanConsume(consumed: seq<()>, produced: seq<Option<R>>, next: ())
+      decreases height
+    {
+      true
+    }
+    ghost predicate CanProduce(consumed: seq<()>, produced: seq<Option<R>>)
+      decreases height
+    {
+      exists producedByWrapped: seq<Option<T>> :: ValidWrappedProduced(produced, producedByWrapped)
+    }
+
+    ghost predicate ValidWrappedProduced(produced: seq<Option<R>>, producedByWrapped: seq<Option<T>>) {
+      && wrappedCanProduce(Seq.Repeat((), |producedByWrapped|), producedByWrapped)
+      && Enumerated(produced) == Seq.Map(f, Enumerated(producedByWrapped))
+    }
+
+    method Invoke(t: ()) returns (r: Option<R>) 
+      requires Valid()
+      requires CanConsume(consumed, produced, t)
+      modifies Repr
+      decreases height
+      ensures Valid()
+      ensures fresh(Repr - old(Repr))
+      ensures consumed == old(consumed) + [t]
+      ensures produced == old(produced) + [r]
+    {
+      assert ConsumesAnything(wrapped);
+      assert wrapped.Valid();
+      assert wrapped.CanProduce(wrapped.consumed, wrapped.produced);
+      var x := wrapped.Invoke(());
+      match x {
+        case Some(v) => r := Some(f(v));
+        case None => r := None;
+      }
+      Repr := {this} + wrapped.Repr;
+      Update(t, r);
+      assert wrapped.produced == old(wrapped.produced) + [x];
+      assert Enumerated(wrapped.produced) == Enumerated(old(wrapped.produced)) + Enumerated([x]);
+      Seq.LemmaMapDistributesOverConcat(f, Enumerated(old(wrapped.produced)), Enumerated([x]));
+    }
+  }
+}
